

IEOR 173 Lecture Notes

Ryan Lin

Contents

Chapter 1

1.1	Lecture 03	2
	Joint Distributions — 2 • Cov + Correlations — 2 • Hat Example — 3 • Start condition (Ch 3) — 3	

Chapter 2

2.1	Lecture 04	5
	Properties of condition expectation — 5	

Chapter 3

3.1	Lecture 05	7
	Packet Transmission (cont) — 7 • Computing Variance: — 7	

Chapter 1

1.1 Lecture 03

1.1.1 Joint Distributions

$$P(x, y) = P(X \leq x, Y \leq y)$$

This is a cumulative distribution for joint distributions.

If $X \perp Y$ (independent), (perpendicular), then the joint distribution is the product of the marginals.
 $P(X, Y) = P(X)P(Y) \forall X, Y$

1.1.2 Cov + Correlations

Covariance is a measure of linear dependence.

$$\text{Cov}(X, Y) = E[(X - EX)(Y - EY)] = EXY - EXEY$$

Interpretation: If they vary together, Cov is larger.

Properties

1. $\text{Cov}(X, X) = \text{Var}(X)$
2. $\text{Cov}(X, Y) = \text{Cov}(Y, X)$
3. $\text{Cov}(cX, Y) = c\text{Cov}(X, Y)$
4. $\text{Cov}(X, Y + Z) = \text{Cov}(X, Y) + \text{Cov}(X, Z)$

Correlation:

$$\rho(X, Y) = \frac{\text{Cov}(X, Y)}{sd(X) \cdot sd(Y)}$$

If

- > 0 , pos correlation
- < 0 , negative correlation
- $= 0$ No correlation

Note:-

Independent does imply uncorrelated, however uncorrelated does not imply independent.

Ex: If $P(-1, 1) = P(0, 0) = P(1, 1) = \frac{1}{3}$. then $E[XY] = \frac{0}{3} = 0$. However, $E[X] = 0, EY = ?$, therefore $E[XY] = 0$ and $\text{Cov}(X, Y) = 0$. There is no linear relationship, however there is a dependency for $y = x^2$.

Therefore, we can generalize our variance formula

$$\text{Var}(A + \sum b_i X_i) = \sum b_i^2 \text{Var}(X_i) + \sum_{\forall i, j, i \neq j} b_i b_j \text{Cov}(X_i, X_j)$$

1.1.3 Hat Example

Example 1.1.1 (Lists of number)

Imagine go to party, men take off hats, women keep on hats. Each man randomly takes a hat and leaves. Let $X = \#$ of matches in N pairs (man and his hat)

What is EX and $Var(X)$?

If two men, the only possibility of matches are 0 and 2. The mean is 1. If three men, a similar pattern occurs.

$$EX = 1 \forall N$$

As N grows larger, the probability decreases, but there is more men to balance it out.

$$Var(X) = 1 \forall N \geq 2$$

We can prove this by using Indicators.

Let $X = \sum^N I_i$, where $I_i = 1$ if it is a match $\sim Bern(\frac{1}{N})$

$$EX = E[\sum I] = \sum^N E[I] = N \frac{1}{N} = 1$$

$$Var(I_i) = E[I^2] - [EI]^2 = p - p^2 = p(1 - p) = \frac{1}{N} - \frac{1}{N^2} = \frac{N-1}{N^2}$$

$$Cov(I_i, I_j) = E[I_i I_j] - EI_i EI_j$$

$$E[I_i I_j] = P(\text{both } i \text{ and } j \text{ match}) = P(I_i = 1, I_j = 1)$$

$$P(I_i = 1)P(I_j = 1 | I_i = 1) = \frac{1}{N} \cdot \frac{1}{N-1}$$

Conceptually, we can think of event j following event i

$$Cov(I_i, I_j) = \frac{1}{n(n-1)} - \left(\frac{1}{n}\right)^2 = \frac{1}{N^2(N-1)}$$

$$Var(X) = Var(\sum I_i) = \sum Var(I_i) + \sum Cov(I_i, I_j) = N \cdot \frac{N-1}{N^2} + N(N-1) \frac{1}{N^2(N-1)} = 1$$

The calculation will be left as an exercise to the future reader.

As $N \rightarrow \infty$,

$$Cov(I_i, I_j) \rightarrow 0$$

$$Var(I_i) \rightarrow \frac{1}{N}$$

$$X \rightarrow Bin(N, \frac{1}{N}) \sim Poisson(1)$$

Intuitively, if there are thousands of men there, whether or not 1 person gets his hat is not really going to affect the chances another gets his.

1.1.4 Start condition (Ch 3)

What if we have dependent random variables and want to compute conditional probabilities?

Conditions:

1. discrete: $P(X, y) = P(X = x, Y = y), P(x, y) = P(X \leq x, Y \leq y) = \sum_{\leq x} \sum_{\leq y} P(x, y)$
2. continuous: $f(x, y) = F(x, y) = \int_{-\infty}^x \int_{-\infty}^y f(u, v) du dv$

3. marginal: $F_X(x) = P(X \leq x) = F(X, \infty)$

4. conditional: $P_{x|y}(X | y) = P(X = x | Y = y) = \frac{P(X=x, Y=y)}{P(Y=y)} = \frac{P_{x,y}(X,y)}{P_y(y)} = \frac{\text{joint}}{\text{marginal}}$

Chapter 2

2.1 Lecture 04

2.1.1 Properties of condition expectation

$$E[X|X = x] = x \forall x$$

$$E[X|Y = y]$$

, is a number bu $E[X|Y]$ is a random variable.

$$X \perp W, X \sim \exp(\lambda), W \sim \exp(\lambda)$$

$$f_x(x) = \lambda e^{-x} \text{ for } x \geq 0$$

$Y = X + W$, condition on $Y = y$, $E[X|Y = y]$. We need $f_{x|y}(x|y)$

$$X|y + W = [y - X|y]$$

This should have the same distributions.

To show this, we need to get the distribution function.

$$f_{x|y}(x|y) \frac{f_{x,y}(x, y)}{f_y(y)} = \frac{f_{x,w}(x, y - x)}{f_y(y)} = \frac{f_x(x)f_w(y - x)}{f_y(y)} = \lambda e^{-\lambda x} \lambda e^{-\lambda(y-x)} = \lambda^2 e^{-\lambda y}$$

For $0 \leq x \leq y$

We also need to get the marginal distributions.

$$f_y(y) = \lambda^2 \int_{-\infty}^{\infty} f_{x,y}(x, y) dx = \lambda^2 \int_0^y e^{-\lambda y} dx = \lambda^2 y e^{-\lambda y}$$

$$f_{x|y}(x|y) = \frac{f_{x,y}(x, y)}{f_y(y)} \frac{\lambda^2 e^{-\lambda y}}{\lambda^2 y e^{-\lambda y}} = \frac{1}{y}$$

This is a uniform distribution from $0 \leq x \leq y$. Therefore $E[X|Y = y] = \int_0^y (x \frac{1}{y}) dx = \frac{y}{2}$

Instead, if we take $G(y) = E[X|Y]$, which is a random variable, we can get $E[E[X|Y]]$.

We can do this by $E[g(Y)] = \int_{-\infty}^{\infty} g(x) D(x) dx$, which is the probability $g(X)$ multiplied by the density $d(x)$.

$$E[E[X|Y]] = \int E[X|Y = y]f_y(y)dy$$

It turns out that this becomes $E[X]$.

Example 2.1.1

$Y = \sum^N X_i, EX_i = \mu, N \perp X_i$'s, or N is independent of the X_i s.

$$\begin{aligned} E[Y] &= E\left[\sum^N y_n\right] = E\left[E\left[\sum^N X_i|N\right]\right] = \sum_{\text{all } n} E\left[\sum^N X_i|N = n\right]p_n(n) = \sum_{\text{all } n} E\left[\sum^N m^n X_1\right]p_n(n) = \sum_{\text{all } n} n\mu p_n(n) \\ &= \mu \sum n p_n(n) = \mu EN \end{aligned}$$

Where N is discrete, integer valued, nonnegative. $p_n(n)$ is the pmf for n

Example 2.1.2 (Mean of a geometric)

$$X \sim \text{geom}(p)$$

Find EX .

Because geometric dists are memoryless, we can condition on the first step.

Let $I = I\{\text{1st trial is a success}\} \sim \text{Bern}(p)$

Compute EX

$$\begin{aligned} EX &= E[E[X|I]] = \sum_{\text{all } i} E[X|I = i]p(I = i) = E[X|I = 1]p(I = 1) + E[X|I = 0]p(I = 0) \\ &= 1p + (1 + EX)(1 - p) \implies EX = \frac{1}{p} \end{aligned}$$

Basically saying, we either get the heads on this trial, or then we have to restart.

Example 2.1.3 (Packet Transmission)

Serve 1 packet per time slot. Each slot we have $A_i = \#$ arrivals in slot i . We assume i.i.d. and has p_0, p_1, p_2 .

We assume that the buffer is size 2. (We can only hold 2 packets in the buffer)

Basically, for every time slot, we can only store up to 2 packets. Each timeslot, one packet leaves the buffer, and if there is too many packets, the incoming packet has to bounce.

N = length of busy period

A busy is period is where there are arrivals to an empty system and ends when the system is emptied again.

Need $E[N]$

First thing that we need to think about is conditioning. It would be helpful to know how many packets start the busy period, therefore we condition on $X = \#$ packets that start the busy period (b.p), where $X \in \{1, 2\}$. Thus we also need to know $P(X = 1) = P(A = 1|A = 1 \text{ or } = 2) = \frac{p_1}{p_1 + p_2}$ and $P(X = 2) = P(A = 2|\dots) = \frac{p_2}{p_1 + p_2}$.

$$E[N] = E[E[N|X]] = E[N|X = 1] \frac{p_1}{p_1 + p_2} + E[N|X = 2] \frac{p_2}{p_1 + p_2}$$

Chapter 3

3.1 Lecture 05

3.1.1 Packet Transmission (cont)

Example 3.1.1 (Packet Transmission (cont))

Packet transmission appends A_i i.i.d. p_0, p_1, p_2 . N = length of busy period. We still want $E[N]$

$$X = \begin{cases} 1 \frac{p_1}{p_1 + p_2} \\ 2 \frac{p_2}{p_1 + p_2} \end{cases}$$

$$E[N] = E[E[N|X]] = E[N|X = 1] \frac{p_1}{p_1 + p_2} + E[N|X = 2] \frac{p_2}{p_1 + p_2}$$

We now need to compute $E[N|X = n]$.

For simplicity $E[N_1] = E[N|X = 1]$:

It would help to know how many packets we get at time 1

$$E[N_1] = E[E[N_1|A]]$$

where A is the number of arrivals in the slot of the busy period.

$$\begin{aligned} E[N] &= E[N_1|A = 0]p_0 + E[N_1|A = 1]p_1 + E[N_1|A = 2]p_2 \\ &= 1p_0 + (1 + E[N_1])p_1 + (1 + E[N_2])p_2 \end{aligned}$$

We can use the $1 + E[N_1]$ because of the i.i.d. and the memory less state.

$$E[N_2] = E[N_2|A = 0]p_0 + E[N_2|A = 1]p_1 + E[N_2|A = 2]p_2$$

$$E[N_2] = (1 + E[N_1])p_0 + (1 + E[N_2])p_1 + (1 + E[N_2])p_2$$

The last term is because the buffer only has storage for 2 packets. If one goes out, then one gets replaced and the other gets sent away.

We can thus solve for $E[N_1]$ and $E[N_2]$, which we can plug into the original equation.

This is a very simple Markov Chain.

3.1.2 Computing Variance:

$\text{Var}(x)$ in two methods

1. Use $\text{Var}(x) = E[X^2] - E[X]^2$, condition for $E[X^2] + E[X]$
2. Condition Var formula

Example for method 1:

$$X \sim \text{geo}(p)$$

$$E[X^2] = E[E[X^2]|I] \text{ where } I = \text{indicator of success} \sim \text{Bern}(p)$$

$$\begin{aligned} E[X^2] &= E[X^2|I=1]p + E[X^2|I=0](1-p) \\ &= 1p + (E[(X+1)^2])(1-p) = p + E[X^2 + 2X + 1](1-p) \\ &= p + (E[X^2] + E[2X] + 1)(1-p) \end{aligned}$$

$$\text{Solve for } E[X^2] = \frac{n-p}{p^2}$$

$$\text{Var}(X) = E[X^2] - (E[X])^2 = \frac{2-p}{p^2} - \left(\frac{1}{p}\right)^2 = \frac{1-p}{p^2}$$

How do we get the method 2 formula?

Proof. Conditional Variance Formula

$$\begin{aligned} [E[\text{Var}(X|Y)] + \text{Var}(E[X|Y])] &= E[E[X|Y]^2] - (E[X|Y])^2 + E[E[X|Y]^2] - E[E[E[X|Y]^2]]^2 \\ &= E[E[X^2|Y]] - E[E[X|Y]]^2 + E[X^2] - E[X]^2 \\ &= \text{Var}(X) \end{aligned}$$

Theorem 3.1.1 $X \perp Y \implies \text{Var}(XY) = \text{Var}(X)$

$$X \perp Y \implies \text{Var}(XY) = E[Y^2] \text{Var}(x) + E[X]^2 \text{Var}(Y) = E[X^2] \text{Var}(Y) + E[Y]^2 \text{Var}(x)$$

$$\text{Var}(XY) = E[\text{Var}(XY|y)] + \text{Var}(E[XY|y])$$

For the first term:

$$\text{Var}(XY|Y=y) = \text{Var}(X_y|Y=y) = y^2 \text{Var}(X) \implies \text{Var}(XY|y) = y^2 \text{Var}(X)$$

We can do this because X is independent of Y .

For the second term:

$$E[XY|Y=y] = yE[X] \implies E[XY|y] = YE[X]$$

Therefore,

$$\text{Var}(XY) = E[Y^2 \text{Var}(X)] + \text{Var}(YE[X]) = \text{Var}(X)E[Y^2] + E[X]^2 \text{Var}(Y)$$

Theorem 3.1.2

X_i is i.i.d. N is an integer valued random variable independent of the X_i s. Find the $\text{Var}(\sum^N X_i)$

$$\text{Var}(\sum^N X_i) = E[\text{Var}(\sum^N X_i|N)] + \text{Var}(E[\sum^N X_i|N])$$

For the first term:

$$\text{Var}(\sum^N X_i|N = n) = \text{Var}(\sum^n X_n|N = n) = \sum^n \text{Var}(X|N = n) = \sum^n \text{Var}(X) = n \text{Var}(X_i)$$

We proved the second term earlier.

$$E[\text{Var}(\sum^N X_i)] = E[N \text{Var}(X_i)] + \text{Var}(NE[X_i]) = E[N] \text{Var}(X_i) + \text{Var}(N)E[X_i]^2$$

If $N \perp X$

$$\text{Var}(NX) = E[X^2] \text{Var}(N) + E[N^2] \text{Var}(X)$$

This one is like the catering example, where everyone orders the same thing. The other is if all the X_i are i.i.d., therefore ordering different things. Therefore the first is more variable than the second.